Make balloc Use all but first bit of first word
be4f286e12 split the bitmap allocator into two levels but wasted space
by not allocating any bits in the first word. This fixes that
shortcoming so no space is wasted at the cost of more computation.

src/Balloc.v
@@ -118,7 +118,7 @@ Module BmpWord (Sig : AllocSig) (WBSig : WordBMapSig).
   Qed.
 
   Definition has_avail (s : state) := if state_dec s then false else true.
-  Definition avail_nonzero s i := if (addr_eq_dec i 0) then false else has_avail s.
+  Definition avail_nonzero s i := if (addr_eq_dec i 0) then (has_avail (s ^| wone _)) else has_avail s.
 
   Lemma HasAvail_has_0 : forall s, HasAvail s -> {i | i < length (bits s) /\ forall d, selN (bits s) i d = avail}.
   Proof.
@@ -203,7 +203,7 @@ Module BmpWord (Sig : AllocSig) (WBSig : WordBMapSig).
     match r with
     | None => Ret ^(ms, None)
     | Some (bn, nonfull) =>
-      match ifind_byte nonfull with
+      match ifind_byte (if addr_eq_dec bn 0 then (nonfull ^| wone _) else nonfull) with
       | None =>
         (* won't happen *) Ret ^(ms, None)
       | Some (i, _) =>
@@ -486,14 +486,75 @@ Module BmpWord (Sig : AllocSig) (WBSig : WordBMapSig).
     auto.
   Qed.
 
-  Lemma avail_nonzero_not_zero : forall bmap i,
-    avail_nonzero (selN bmap i $0) i = true -> i <> 0.
+  Lemma bits_wor_wone : forall sz (w : word (S sz)),
+    bits (w ^| wone _) = inuse :: bits (wtl w).
   Proof.
-    unfold avail_nonzero; intros.
-    destruct (addr_eq_dec i 0); congruence.
+    intros.
+    destruct (shatter_word_S w); repeat deex.
+    rewrite wor_wone.
+    rewrite bits_cons.
+    reflexivity.
   Qed.
 
-  Local Hint Resolve avail_nonzero_is_avail avail_nonzero_not_zero.
+  Lemma avail_nonzero_first_is_avail : forall bmap ii b d d',
+    length bmap > 0 ->
+    ifind_byte (selN bmap 0 d' ^| wone _) = Some (ii, b) ->
+    Avail (selN (to_bits bmap) ii d).
+  Proof.
+    unfold ifind_byte.
+    unfold Defs.itemsz. simpl.
+    generalize (WBSig.word_size_nonzero).
+    generalize WBSig.word_size.
+    unfold avail_nonzero; intros.
+    unfold Avail.
+    denote (ifind_list _ _ _ = _) as Hl.
+    apply ifind_list_ok_bound in Hl as ?; simpl in *.
+    rewrite bits_length in *.
+    rewrite selN_to_bits by auto.
+    rewrite Nat.div_small by auto.
+    rewrite Nat.mod_small by auto.
+    apply ifind_list_ok_cond in Hl as ?.
+    simpl in *.
+    destruct weq; subst; try congruence.
+    eapply ifind_list_ok_item in Hl as ?.
+    simpl in *.
+    rewrite Nat.sub_0_r in *.
+    destruct n; try congruence.
+    rewrite bits_wor_wone in *.
+    destruct ii; simpl in H0.
+    compute [selN inuse avail natToWord mod2] in *. congruence.
+    match goal with |- context [selN ?l 0 ?d] =>
+      rewrite selN_inb with (d1 := d') (d2 := d) in H3;
+      pose proof (shatter_word_S (selN l 0 d)); repeat deex
+    end.
+    denote (selN _ _ _ = _) as Hx.
+    rewrite Hx in *.
+    rewrite bits_cons.
+    simpl in *.
+    erewrite selN_inb by (rewrite bits_length; omega). eauto.
+    Unshelve.
+    all : eauto; solve [exact nil | exact None].
+  Qed.
+
+  Lemma ifind_byte_first_not_zero : forall (w : state) b,
+    ifind_byte (w ^| wone _) = Some (0, b) -> False.
+  Proof.
+    unfold ifind_byte, state.
+    generalize (WBSig.word_size_nonzero).
+    unfold Defs.itemsz. simpl.
+    generalize WBSig.word_size.
+    intros n H' w b H.
+    eapply ifind_list_ok_cond in H as Ha.
+    eapply ifind_list_ok_item in H as Hb.
+    cbn in *.
+    destruct n; try congruence.
+    rewrite bits_wor_wone in *.
+    simpl in *.
+    destruct weq; compute in *; congruence.
+    Unshelve. eauto.
+  Qed.
+
+  Local Hint Resolve avail_nonzero_is_avail avail_nonzero_first_is_avail ifind_byte_first_not_zero.
 
   Lemma avail_item0 : forall n d, n < Defs.itemsz -> Avail (selN (bits Bmp.Defs.item0) n d).
   Proof.
@@ -577,14 +638,13 @@ Module BmpWord (Sig : AllocSig) (WBSig : WordBMapSig).
     induction n; simpl; f_equal; auto.
   Qed.
 
-  Lemma ifind_byte_inb : forall l i n b d,
-    i < length l ->
-    ifind_byte (selN l i d) = Some (n, b) ->
+  Lemma ifind_byte_inb : forall x n b,
+    ifind_byte x = Some (n, b) ->
     n < Defs.itemsz.
   Proof.
     unfold ifind_byte.
     intros.
-    apply ifind_list_ok_bound in H0.
+    apply ifind_list_ok_bound in H.
     rewrite bits_length in *.
     simpl in *. auto.
   Qed.
@@ -712,16 +772,17 @@ Module BmpWord (Sig : AllocSig) (WBSig : WordBMapSig).
     contradict Hc; pred_apply; cancel.
 
     eapply is_avail_in_freelist; eauto.
+    destruct addr_eq_dec; subst; eauto.
     rewrite to_bits_length; apply bound_offset; auto.
     denote (ifind_byte _ = Some _) as Hb.
-    apply ifind_byte_inb in Hb; auto.
-    eapply avail_nonzero_not_zero; eauto.
+    apply ifind_byte_inb in Hb as Hc; auto.
     rewrite Nat.eq_add_0, Nat.eq_mul_0 in *.
-    intuition (auto || exfalso; auto).
+    intuition (subst; exfalso; try destruct addr_eq_dec; eauto).
     eapply bmap_rep_length_ok1; eauto.
     rewrite to_bits_length, length_updN.
     apply bound_offset; auto.
     eapply is_avail_in_freelist; eauto.
+    destruct addr_eq_dec; subst; eauto.
     rewrite to_bits_length; apply bound_offset; auto.
     Unshelve.
     all : solve [auto | exact full].
